`StateGettersSummary`: add `TIMESTAMP` summary proofs

EvmEquivalence/Summaries/StateGettersSummary.lean
@@ -15,13 +15,14 @@ inductive stateGetter_op where
 | caller
 | gasprice
 | coinbase
+| timestamp
 deriving BEq, DecidableEq
 
 section
 
 variable (op : stateGetter_op)
 variable (word₁ word₂ word₃: UInt256)
-variable (gas gasCost symGasPrice: ℕ)
+variable (gas gasCost symGasPrice symTimestamp : ℕ)
 variable (symStack : Stack UInt256)
 variable (symPc symGasAvailable symRefund symActiveWords : UInt256)
 variable (symExecLength : ℕ)
@@ -38,13 +39,14 @@ abbrev originEVM := @Operation.ORIGIN .EVM
 abbrev callerEVM := @Operation.CALLER .EVM
 abbrev gaspriceEVM := @Operation.GASPRICE .EVM
 abbrev coinbaseEVM := @Operation.COINBASE .EVM
+abbrev timestampEVM := @Operation.TIMESTAMP .EVM
 
 abbrev address_instr : Option (Operation .EVM × Option (UInt256 × Nat)) := some ⟨addressEVM, none⟩
 abbrev origin_instr : Option (Operation .EVM × Option (UInt256 × Nat)) := some ⟨originEVM, none⟩
 abbrev caller_instr : Option (Operation .EVM × Option (UInt256 × Nat)) := some ⟨callerEVM, none⟩
 abbrev gasprice_instr : Option (Operation .EVM × Option (UInt256 × Nat)) := some ⟨gaspriceEVM, none⟩
 abbrev coinbase_instr : Option (Operation .EVM × Option (UInt256 × Nat)) := some ⟨coinbaseEVM, none⟩
-
+abbrev timestamp_instr : Option (Operation .EVM × Option (UInt256 × Nat)) := some ⟨timestampEVM, none⟩
 
 @[simp]
 def stateGetter_op.get : (Option (Operation .EVM × Option (UInt256 × Nat))) :=
@@ -54,6 +56,7 @@ def stateGetter_op.get : (Option (Operation .EVM × Option (UInt256 × Nat))) :=
   | .caller => caller_instr
   | .gasprice => gasprice_instr
   | .coinbase => coinbase_instr
+  | .timestamp => timestamp_instr
 
 --@[simp]
 def stateGetter_op.t : Operation .EVM :=
@@ -63,6 +66,7 @@ def stateGetter_op.t : Operation .EVM :=
   | .caller  => (caller_instr.get rfl).1
   | .gasprice  => (gasprice_instr.get rfl).1
   | .coinbase  => (coinbase_instr.get rfl).1
+  | .timestamp  => (timestamp_instr.get rfl).1
 
 def EVM.step_arith : Transformer := EVM.step gas gasCost op.get
 
@@ -74,8 +78,9 @@ def stateGetter_op.do (symState : EVM.State) :=
   | .address  => UInt256.ofNat ↑symState.executionEnv.codeOwner
   | .origin  => UInt256.ofNat ↑symState.executionEnv.sender
   | .caller  => UInt256.ofNat ↑symState.executionEnv.source
-  | .gasprice  => UInt256.ofNat ↑symState.executionEnv.gasPrice
+  | .gasprice  => UInt256.ofNat symState.executionEnv.gasPrice
   | .coinbase  => UInt256.ofNat ↑symState.coinBase
+  | .timestamp  => symState.timeStamp
 
 /- theorem EvmYul.step_op_summary (symState : EVM.State):
   EvmYul.step_arith op {symState with
@@ -99,6 +104,7 @@ theorem EVM.step_add_to_step_add (gpos : 0 < gas) (symState : EVM.State):
                   gasPrice := symGasPrice,
                   header := {symState.executionEnv.header with
                     beneficiary := symCoinbase
+                    timestamp := symTimestamp
                   }
                   perm := symPerm},
       accountMap := symAccounts,
@@ -136,6 +142,7 @@ theorem EVM.step_getter_summary (gpos : 0 < gas) (symState : EVM.State):
                   gasPrice := symGasPrice,
                   header := {symState.executionEnv.header with
                     beneficiary := symCoinbase
+                    timestamp := symTimestamp
                   }
                   perm := symPerm},
       accountMap := symAccounts,
@@ -165,6 +172,7 @@ def stateGetter_op.to_bin : ByteArray :=
   | .caller  => ⟨#[0x33]⟩
   | .gasprice => ⟨#[0x3A]⟩
   | .coinbase => ⟨#[0x41]⟩
+  | .timestamp => ⟨#[0x42]⟩
 
 @[simp]
 theorem decode_singleton_address :
@@ -181,6 +189,9 @@ theorem decode_singleton_gasprice :
 @[simp]
 theorem decode_singleton_coinbase :
   decode ⟨#[0x41]⟩ (.ofNat 0) = some ⟨coinbaseEVM, none⟩ := rfl
+@[simp]
+theorem decode_singleton_timestamp :
+  decode ⟨#[0x42]⟩ (.ofNat 0) = some ⟨timestampEVM, none⟩ := rfl
 
 @[simp]
 theorem decode_singleton :
@@ -222,6 +233,7 @@ theorem X_getter_summary
                   gasPrice := symGasPrice,
                   header := {symState.executionEnv.header with
                     beneficiary := symCoinbase
+                    timestamp := symTimestamp
                   }
                   perm := symPerm},
     accountMap := symAccounts,
@@ -258,7 +270,7 @@ theorem X_getter_summary
   have gPos : (0 < g_pos) := by
     revert enoughGas; simp [stateGetter_op.C'_comp]
     cases op <;> aesop (add safe (by omega))
-  have step_rw (cost : ℕ) := (EVM.step_getter_summary op g_pos cost symGasPrice symStack (.ofNat 0) symGasAvailable symRefund symActiveWords symExecLength symReturnData op.to_bin symMemory symAccessedStorageKeys symAccounts symCodeOwner symSender symSource symCoinbase symPerm gPos)
+  have step_rw (cost : ℕ) := (EVM.step_getter_summary op g_pos cost symGasPrice symTimestamp symStack (.ofNat 0) symGasAvailable symRefund symActiveWords symExecLength symReturnData op.to_bin symMemory symAccessedStorageKeys symAccounts symCodeOwner symSender symSource symCoinbase symPerm gPos)
   have stack_ok_rw : (1024 < List.length symStack + 1) = False := by
     cases op <;> aesop (add safe (by omega))
   cases cop: op <;>
